openmls/proofs/lean/Openmls/Extraction/ProofObligations.lean
@@ -93,6 +93,12 @@ theorem binary_tree.array_representation.treemath.is_node_in_tree.spec.proof
   := by sorry
 
 @[spec]
+theorem binary_tree.array_representation.treemath.LeafNodeIndex.new.spec.proof
+   (index : Std.U32) :
+  binary_tree.array_representation.treemath.LeafNodeIndex.new.spec index
+  := by sorry
+
+@[spec]
 theorem
   binary_tree.array_representation.treemath.LeafNodeIndex.to_tree_index.spec.proof
    (self : binary_tree.array_representation.treemath.LeafNodeIndex) :
@@ -106,6 +112,13 @@ theorem
    (node_index : Std.U32) :
   binary_tree.array_representation.treemath.LeafNodeIndex.from_tree_index.spec
   node_index
+  := by sorry
+
+@[spec]
+theorem
+  binary_tree.array_representation.treemath.ParentNodeIndex.new.spec.proof
+   (index : Std.U32) :
+  binary_tree.array_representation.treemath.ParentNodeIndex.new.spec index
   := by sorry
 
 @[spec]
